\newpage
Energía cinética
\[T=\frac{1}{2}m_1(\dot x_1+\dot y_1)+\frac{1}{2}m_2(\dot x_2+\dot y_2)\]\\
\[\dot x_1^2=\frac{S_1^2}{4}\dot\theta_1^2\cos^2\theta_1\]
\[\dot y_1^2=\frac{S_1^2}{4}\dot\theta_1^2\sin^2\theta_1\]
\[\dot x_2^2=(S_1\dot\theta_1\cos\theta_1+l_2\dot\theta_2\cos\theta_2)^2\to\dot x_2^2=S_1^2\dot\theta_1^2\cos^2\theta_1+l_2^2\dot\theta_2^2\cos^2\theta_2+2S_1l_2\dot\theta_1\dot\theta_2\cos\theta_1\cos\theta_2\]
\[\dot y_2^2=(S_1\dot\theta_1\sin\theta_1+l_2\dot\theta_2\sin\theta_2)^2\to\dot y_2^2=S_1^2\dot\theta_1^2\sin^2\theta_1+l_2^2\dot\theta_2^2\sin^2\theta_2+2S_1l_2\dot\theta_1\dot\theta_2\sin\theta_1\sin\theta_2\]\\

\[T=\frac{1}{2}m_1\left(\frac{S_1^2}{4}\dot\theta_1^2\cos^2\theta_1+\frac{S_1^2}{4}\dot\theta_1^2\sin^2\theta_1\right)+\]
\[\frac{1}{2}m_2\left(S_1^2\dot\theta_1^2\cos^2\theta_1+l_2^2\dot\theta_2^2\cos^2\theta_2+2S_1l_2\dot\theta_1\dot\theta_2\cos\theta_1\cos\theta_2+\right\]
\[\left S_1^2\dot\theta_1^2\sin^2\theta_1+l_2^2\dot\theta_2^2\sin^2\theta_2+2S_1l_2\dot\theta_1\dot\theta_2\sin\theta_1\sin\theta_2\right)\]\\

\[T=\frac{1}{2}m_1\left(\frac{S_1^2}{4}\dot\theta_1^2\cos^2\theta_1+\frac{S_1^2}{4}\dot\theta_1^2\sin^2\theta_1\right)+\]
\[\frac{1}{2}m_2\left(S_1^2\dot\theta_1^2+l_2^2\dot\theta_2^2+2S_1l_2\dot\theta_1\dot\theta_2\cos\theta_1\cos\theta_2+2S_1l_2\dot\theta_1\dot\theta_2\sin\theta_1\sin\theta_2\right)\]


\newpage
Energía cinética\\
Producto de cosenos
\[\cos a\cos b=\frac{1}{2}\left[cos(a+b)+cos(a-b)\right]\]
Producto de senos
\[\sin a\sin b=\frac{1}{2}\left[cos(a-b)-cos(a+b)\right]\]\\
\[T=\frac{1}{2}m_1\left(\frac{S_1^2}{4}\dot\theta_1^2\cos^2\theta_1+\frac{S_1^2}{4}\dot\theta_1^2\sin^2\theta_1\right)+\frac{1}{2}m_2\left(S_1^2\dot\theta_1^2+l_2^2\dot\theta_2^2+2S_1l_2\dot\theta_1\dot\theta_2\cos(\theta_1-\theta_2)\right)\]\\

\[T=m_1\frac{S_1^2}{8}\dot\theta_1^2\cos^2\theta_1+m_1\frac{S_1^2}{8}\dot\theta_1^2\sin^2\theta_1+\frac{1}{2}m_2S_1^2\dot\theta_1^2+\frac{1}{2}m_2l_2^2\dot\theta_2^2+m_2S_1l_2\dot\theta_1\dot\theta_2\cos(\theta_1-\theta_2)\]
